LeanZX.lean
@@ -8,5 +8,6 @@ import LeanZX.Tactics
 import LeanZX.Rules.SpiderFusion
 import LeanZX.Rules.IdentityRemoval
 import LeanZX.Rules.HadamardHadamard
+import LeanZX.Rules.ColourChange
 import LeanZX.DerivedRules.PiPi
 import LeanZX.Examples
