LeanZX/Rules/ColourChange.lean
@@ -1,0 +1,38 @@
+import LeanZX.Axioms
+import LeanZX.Tactics
+
+open Lean Elab Tactic Meta
+
+def ZXDiagram.colourChange (d: ZXDiagram) (a : NodeId) : Except String ZXDiagram := do
+  -- Get node info
+  let nodeA ← (d.getNode? a).toExcept s!"Node {a} not found"
+  let colorA ← (Node.color? nodeA).toExcept s!"Node {a} is not a spider"
+  let phaseA ← (Node.phase? nodeA).toExcept s!"Node {a} has no phase"
+  let aNeighbors := d.neighbors a
+  -- Flip node colour
+  let newColour := if colorA == SpiderColor.X then SpiderColor.Z else SpiderColor.X
+  let aColourChanged := Node.spider newColour phaseA
+  let d := d.setNode a aColourChanged
+  -- Add Hadamards
+  let (d, hadIds) := d.addNodes (aNeighbors.map (λ _ => Node.hadamard))
+  -- Rewire edges
+  let d := d.removeEdgesOf a
+  let d := d.addEdges (hadIds.map (λ had => Edge.mk had a))
+  let d := d.addEdges (aNeighbors.zipWith (Edge.mk . .) hadIds)
+  return d.normalize
+
+namespace LeanZX
+
+axiom ZXDiagram.colourChange_sound (d : ZXDiagram) (a : NodeId) (d' : ZXDiagram) :
+  d.colourChange a = .ok d' → d ≈z d'
+
+/-- Swap the colour of a Z or X spider, and surround it with Hadamards. Shows the resulting diagram. -/
+syntax "zx_cc" num : tactic
+
+elab_rules : tactic
+  | `(tactic| zx_cc $a) =>
+    applyRewrite a "Colour Change"
+      ``ZXDiagram.colourChange ``ZXDiagram.colourChange_sound
+      #[mkNatLit a.getNat]
+
+end LeanZX
